chore: alignment of Array.any/all lemmas with List (#6353)
This PR reproduces the API around `List.any/all` for `Array.any/all`.

src/Init/Data/Array/Basic.lean
@@ -663,7 +663,7 @@ def all (as : Array α) (p : α → Bool) (start := 0) (stop := as.size) : Bool 
   Id.run <| as.allM p start stop
 
 def contains [BEq α] (as : Array α) (a : α) : Bool :=
-  as.any (· == a)
+  as.any (a == ·)
 
 def elem [BEq α] (a : α) (as : Array α) : Bool :=
   as.contains a
